theories/prophecy/syn_type.v
@@ -1,52 +1,38 @@
 Require Import ssreflect.
 From stdpp Require Import prelude.
-From lrust.util Require Import fancy_lists.
+From lrust.util Require Import basic fancy_lists.
 Set Default Proof Using "Type".
 
 (** * Syntax for Coq type *)
 
-Inductive syn_type0 := Zₛ | boolₛ | unitₛ | Propₛ.
-Inductive syn_type1 := optionₛ' | listₛ'.
-Inductive syn_type2 := prodₛ' | sumₛ' | funₛ'.
-Inductive syn_typex := xprodₛ' | xsumₛ'.
-
-Instance syn_type0_eq_dec: EqDecision syn_type0. Proof. solve_decision. Qed.
-Instance syn_type1_eq_dec: EqDecision syn_type1. Proof. solve_decision. Qed.
-Instance syn_type2_eq_dec: EqDecision syn_type2. Proof. solve_decision. Qed.
-Instance syn_typex_eq_dec: EqDecision syn_typex. Proof. solve_decision. Qed.
-
-Inductive syn_type :=
-| SynType0:> syn_type0 → syn_type
-| SynType1: syn_type1 → syn_type → syn_type
-| SynType2: syn_type2 → syn_type → syn_type → syn_type
-| SynTypex: syn_typex → list syn_type → syn_type.
+Inductive syn_type := Zₛ | boolₛ | unitₛ | empty_setₛ | Propₛ
+| optionₛ (_: syn_type) | listₛ (_: syn_type)
+| prodₛ (_ _: syn_type) | sumₛ (_ _: syn_type) | funₛ (_ _: syn_type)
+| xprodₛ (_: list syn_type) | xsumₛ (_: list syn_type).
 
 Implicit Type 𝔄 𝔅: syn_type.
 
-Local Notation all2 f := (fix all2 xl yl := match xl, yl with | [], [] => true
+Local Notation all2 f := (fix all2 xl yl := match xl, yl with [], [] => true
   | x :: xl', y :: yl' => f x y && all2 xl' yl' | _, _ => false end).
 
-Fixpoint syn_type_beq (𝔄 𝔅: syn_type) : bool :=
-  match 𝔄, 𝔅 with
-  | SynType0 a, SynType0 b => bool_decide (a = b)
-  | SynType1 f 𝔄, SynType1 g 𝔅 => bool_decide (f = g) && syn_type_beq 𝔄 𝔅
-  | SynType2 f 𝔄 𝔄', SynType2 g 𝔅 𝔅' =>
-      bool_decide (f = g) && syn_type_beq 𝔄 𝔅 && syn_type_beq 𝔄' 𝔅'
-  | SynTypex f 𝔄l, SynTypex g 𝔅l => bool_decide (f = g) && all2 syn_type_beq 𝔄l 𝔅l
+Fixpoint syn_type_beq (𝔄 𝔅: syn_type) : bool := match 𝔄, 𝔅 with
+  | Zₛ, Zₛ | boolₛ, boolₛ | unitₛ, unitₛ | empty_setₛ, empty_setₛ | Propₛ, Propₛ => true
+  | optionₛ 𝔄₀, optionₛ 𝔅₀ | listₛ 𝔄₀, listₛ 𝔅₀ => syn_type_beq 𝔄₀ 𝔅₀
+  | prodₛ 𝔄₀ 𝔄₁, prodₛ 𝔅₀ 𝔅₁ | sumₛ 𝔄₀ 𝔄₁, sumₛ 𝔅₀ 𝔅₁ | funₛ 𝔄₀ 𝔄₁, funₛ 𝔅₀ 𝔅₁
+    => syn_type_beq 𝔄₀ 𝔅₀ && syn_type_beq 𝔄₁ 𝔅₁
+  | xprodₛ 𝔄l, xprodₛ 𝔅l | xsumₛ 𝔄l, xsumₛ 𝔅l => all2 syn_type_beq 𝔄l 𝔅l
   | _, _ => false
   end.
 
 Lemma syn_type_eq_correct (𝔄 𝔅: syn_type) : syn_type_beq 𝔄 𝔅 ↔ 𝔄 = 𝔅.
 Proof.
-  move: 𝔄 𝔅. fix FIX 1. move=> [?|??|???|? 𝔄l] [?|??|???|? 𝔅l]//=;
-  rewrite ?andb_True bool_decide_spec ?FIX.
-  - split; by [move=> ->|move=> [=]].
-  - split; by [move=> [->->]|move=> [=]].
-  - split; [by move=> [[->->]->]|by move=> [=]].
-  - suff ->: ∀𝔄l 𝔅l, all2 syn_type_beq 𝔄l 𝔅l ↔ 𝔄l = 𝔅l.
-    { split; by [move=> [->->]|move=> [=]]. }
-    elim=> [|?? IH][|??]//. rewrite andb_True FIX IH.
-    split; by [move=> [->->]|move=> [=]].
+  move: 𝔄 𝔅. fix FIX 1.
+  have FIXl: ∀𝔄l 𝔅l, all2 syn_type_beq 𝔄l 𝔅l ↔ 𝔄l = 𝔅l.
+  { elim=> [|?? IH][|??]//. rewrite andb_True FIX IH.
+    split; by [move=> [->->]|move=> [=]]. }
+  move=> [|||||?|?|??|??|??|?|?] [|||||?|?|??|??|??|?|?]//=;
+  rewrite ?andb_True ?FIX ?FIXl; try (by split; [move=> ->|move=> [=]]);
+  by split; [move=> [->->]|move=> [=]].
 Qed.
 Instance syn_type_beq_dec: EqDecision syn_type.
 Proof.
@@ -57,24 +43,93 @@ Qed.
 Declare Scope syn_type_scope.
 Bind Scope syn_type_scope with syn_type.
 Delimit Scope syn_type_scope with TYPE.
-Notation optionₛ := (SynType1 optionₛ'). Notation listₛ := (SynType1 listₛ').
-Notation prodₛ := (SynType2 prodₛ'). Notation sumₛ := (SynType2 sumₛ').
-Notation funₛ := (SynType2 funₛ').
 Infix "*" := prodₛ : syn_type_scope. Infix "+" := sumₛ : syn_type_scope.
 Infix "→" := funₛ : syn_type_scope.
-Notation xprodₛ := (SynTypex xprodₛ'). Notation xsumₛ := (SynTypex xsumₛ').
 Notation "Π!" := xprodₛ : syn_type_scope. Notation "Σ!" := xsumₛ : syn_type_scope.
 
 Local Notation tmap' f := (fix tmap' xl :=
   match xl with [] => ^[] | x :: xl' => f x ^:: tmap' xl' end).
 
 Fixpoint of_syn_type (𝔄: syn_type) : Type := match 𝔄 with
-| Zₛ => Z | boolₛ => bool | unitₛ => unit | Propₛ => Prop
-| optionₛ 𝔄 => option (of_syn_type 𝔄) | listₛ 𝔄 => list (of_syn_type 𝔄)
-| prodₛ 𝔄 𝔅 => of_syn_type 𝔄 * of_syn_type 𝔅
-| sumₛ 𝔄 𝔅 => of_syn_type 𝔄 + of_syn_type 𝔅
-| funₛ 𝔄 𝔅 => of_syn_type 𝔄 → of_syn_type 𝔅
-| xprodₛ 𝔄l => Π! (tmap' of_syn_type 𝔄l)
-| xsumₛ 𝔄l => Σ! (tmap' of_syn_type 𝔄l)
-end.
+  | Zₛ => Z | boolₛ => bool | unitₛ => unit | empty_setₛ => ∅ | Propₛ => Prop
+  | optionₛ 𝔄₀ => option (of_syn_type 𝔄₀) | listₛ 𝔄₀ => list (of_syn_type 𝔄₀)
+  | prodₛ 𝔄₀ 𝔄₁ => of_syn_type 𝔄₀ * of_syn_type 𝔄₁
+  | sumₛ 𝔄₀ 𝔄₁ => of_syn_type 𝔄₀ + of_syn_type 𝔄₁
+  | funₛ 𝔄₀ 𝔄₁ => of_syn_type 𝔄₀ → of_syn_type 𝔄₁
+  | xprodₛ 𝔄l => Π! (tmap' of_syn_type 𝔄l)
+  | xsumₛ 𝔄l => Σ! (tmap' of_syn_type 𝔄l)
+  end.
 Coercion of_syn_type: syn_type >-> Sortclass.
+
+Local Notation all f := (fix all xl := match xl with
+  [] => true | x :: xl' => f x && all xl' end).
+Local Notation some f := (fix all xl := match xl with
+  [] => false | x :: xl' => f x || all xl' end).
+
+Fixpoint inh_syn_type (𝔄: syn_type) : bool := match 𝔄 with
+  | prodₛ 𝔄₀ 𝔄₁ => inh_syn_type 𝔄₀ && inh_syn_type 𝔄₁
+  | sumₛ 𝔄₀ 𝔄₁ => inh_syn_type 𝔄₀ || inh_syn_type 𝔄₁
+  | funₛ 𝔄₀ 𝔄₁ => negb (inh_syn_type 𝔄₀) || inh_syn_type 𝔄₁
+  | xprodₛ 𝔄l => all inh_syn_type 𝔄l | xsumₛ 𝔄l => some inh_syn_type 𝔄l
+  | empty_setₛ => false | _ => true
+  end.
+
+Lemma negb_andb b c : negb (b && c) = negb b || negb c.
+Proof. by case b; case c. Qed.
+Lemma negb_orb b c : negb (b || c) = negb b && negb c.
+Proof. by case b; case c. Qed.
+Lemma negb_negb_orb b c : negb (negb b || c) = b && negb c.
+Proof. by case b; case c. Qed.
+
+Lemma of_just_and_neg_inh_syn_type {𝔄: syn_type} :
+  (inh_syn_type 𝔄 → 𝔄) * (negb (inh_syn_type 𝔄) → 𝔄 → ∅).
+Proof.
+  move: 𝔄. fix FIX 1. move=> 𝔄. split.
+  - case: 𝔄=>//= [|||?|?|??|𝔄?|𝔄?|𝔄l|𝔄l]=> H;
+    [exact 0|exact true|exact True|exact None|exact []| | | | |].
+    + move: H=> /andb_True[??]. constructor; by apply FIX.
+    + move: H. case Eq: (inh_syn_type 𝔄); rewrite/= -/inh_syn_type=> H.
+      { apply inl, FIX. by rewrite Eq. } { by apply inr, FIX. }
+    + move: H. case Eq: (inh_syn_type 𝔄)=>/= ??; [by apply FIX|].
+      suff E: Empty_set by done. eapply FIX; [|done]. by rewrite Eq.
+    + move: H. elim 𝔄l; [move=> ?; exact -[]|]=> ?? IH /andb_True [??].
+      split; by [apply FIX|apply IH].
+    + move: H. elim 𝔄l; [done|]=> 𝔄 ? IH.
+      case Eq: (inh_syn_type 𝔄); rewrite/= -/inh_syn_type=> H.
+      { apply xinhd, FIX. by rewrite Eq. } { by apply xintl, IH. }
+  - case: 𝔄=>//= [𝔄?|𝔄?|𝔄?|𝔄l|𝔄l].
+    + rewrite negb_andb. case Eq: (inh_syn_type 𝔄)=>/= ?[a?]; [by eapply FIX|].
+      eapply FIX; [|apply a]. by rewrite Eq.
+    + rewrite negb_orb=> /andb_True[??] [x|x]; eapply FIX; [|apply x| |apply x]=>//.
+    + rewrite negb_negb_orb=> /andb_True[N N'] f. eapply FIX; [done|]. by apply f, FIX.
+    + elim 𝔄l; [done|]=> 𝔄 ? IH. rewrite negb_andb. case Eq: (inh_syn_type 𝔄)
+      =>/= ?[??]; [by apply IH|]. eapply FIX; [|done]. by rewrite Eq.
+    + elim 𝔄l; [move=> ?; by apply absurd|]=> ?? IH. rewrite negb_orb
+      => /andb_True[??] /xsum_cons_to_sum[?|?]; by [eapply FIX|apply IH].
+Qed.
+Lemma of_inh_syn_type {𝔄: syn_type} : inh_syn_type 𝔄 → 𝔄.
+Proof. apply of_just_and_neg_inh_syn_type. Qed.
+Lemma of_neg_inh_syn_type {𝔄: syn_type} : negb (inh_syn_type 𝔄) → 𝔄 → ∅.
+Proof. apply of_just_and_neg_inh_syn_type. Qed.
+
+Lemma to_inh_syn_type {𝔄: syn_type} (x: 𝔄) : inh_syn_type 𝔄.
+Proof.
+  move: 𝔄 x. fix FIX 1. case=>//= [??|??|𝔄?|𝔄l|𝔄l].
+  - move=> [??]. rewrite andb_True. by split; apply FIX.
+  - move=> [?|?]; rewrite orb_True; [left|right]; by apply FIX.
+  - move=> f. case Eq: (inh_syn_type 𝔄); [|done].
+    apply FIX, f, of_inh_syn_type. by rewrite Eq.
+  - elim 𝔄l; [done|]=>/= ?? IH [??]. rewrite andb_True. split; by [apply FIX|apply IH].
+  - elim 𝔄l; [by apply absurd|]=> ?? IH /xsum_cons_to_sum[?|?];
+    rewrite orb_True; [left|right]; by [eapply FIX|apply IH].
+Qed.
+
+Definition syn_typei: Type := { 𝔄 | inh_syn_type 𝔄 }.
+Definition of_syn_typei (𝔄i: syn_typei) : Type := `𝔄i.
+Coercion of_syn_typei: syn_typei >-> Sortclass.
+
+Lemma syn_typei_eq (𝔄i 𝔅i: syn_typei) : 𝔄i = 𝔅i ↔ `𝔄i = `𝔅i.
+Proof. apply (sig_eq_pi _). Qed.
+
+Global Instance syn_typei_inhabited (𝔄i: syn_typei) : Inhabited 𝔄i.
+Proof. apply populate. case 𝔄i=>??. by apply of_inh_syn_type. Qed.
