theories/typing/sum.v
@@ -123,7 +123,7 @@ Section sum.
   Qed.
 
   Definition sum_ty {A B} (ty: type A) (ty': type B) : type (A + B) :=
-    <{xsum_to_sum}> (xsum_ty +[ty; ty']).
+    <{xsum_2_to_sum}> (xsum_ty +[ty; ty']).
 
   Global Instance sum_ty_ne {A B} : NonExpansive2 (@sum_ty A B).
   Proof.
