theories/util/functional_choice.v
@@ -1,3 +1,0 @@
-Require Import ChoiceFacts.
-
-Axiom inhabited_forall_commute: InhabitedForallCommute.
