theories/util/proof_irrelevance.v
@@ -1,4 +1,0 @@
-Require Import ssreflect ProofIrrelevance.
-
-Ltac proof_subst x y :=
-  (have ?: x = y by apply proof_irrelevance); subst x.
